Figured out a way of formalizing minimality of laws. Defined the FreeT monad transformer and proved that RWST is a monad transformer. Reintroduced the definition of monads based on monadic composition and refactored Theory/.

Control/MonadTrans.v
@@ -8,8 +8,8 @@ Require Export HSLib.Control.Monad.
 Class MonadTrans (T : (Type -> Type) -> Type -> Type) : Type :=
 {
     is_monad : forall (M : Type -> Type), Monad M -> Monad (T M);
-    lift : forall {M : Type -> Type} {_inst : Monad M} {A : Type},
-      M A -> T M A;
+    lift :
+      forall {M : Type -> Type} {_inst : Monad M} {A : Type}, M A -> T M A;
     lift_pure :
       forall (M : Type -> Type) {_inst : Monad M} (A : Type) (x : A),
         lift (pure x) = pure x;
