Control/Monoidal.v
@@ -11,27 +11,6 @@ Definition par
 
 Notation "f *** g" := (par f g) (at level 40).
 
-Lemma par_id :
-  forall (A B : Type), @id A *** @id B = id.
-Proof.
-  intros. unfold par, id. ext p. destruct p. reflexivity.
-Qed.
-
-Lemma comp_par_par :
-  forall (A B C A' B' C' : Type)
-  (f1 : A -> B) (f2 : B -> C) (g1 : A' -> B') (g2 : B' -> C'),
-    (f1 *** g1) .> (f2 *** g2) = (f1 .> f2) *** (g1 .> g2).
-Proof.
-  intros. unfold compose, par. ext p. destruct p. reflexivity.
-Qed.
-
-Lemma par_comp :
-  forall (A B A' B' X : Type) (f : A -> B) (g : A' -> B') (h : B * B' -> X),
-    (f *** g) .> h = fun p : A * A' => h (f (fst p), g (snd p)).
-Proof.
-  intros. unfold compose, par. ext p. destruct p. cbn. reflexivity.
-Qed.
-
 (* An alternative characterization of applicative functors as lax monoidal
    functors (or rather, strong monoidal functors, because in the category
    of Coq's types and functions all monoidal functors are strong. *)
@@ -57,3 +36,24 @@ Class isMonoidal (F : Type -> Type) : Type :=
 }.
 
 Hint Rewrite @pairF_default_l @pairF_default_r @pairF_assoc : monoidal.
+
+Lemma par_id :
+  forall (A B : Type), @id A *** @id B = id.
+Proof.
+  intros. unfold par, id. ext p. destruct p. reflexivity.
+Qed.
+
+Lemma comp_par_par :
+  forall (A B C A' B' C' : Type)
+  (f1 : A -> B) (f2 : B -> C) (g1 : A' -> B') (g2 : B' -> C'),
+    (f1 *** g1) .> (f2 *** g2) = (f1 .> f2) *** (g1 .> g2).
+Proof.
+  intros. unfold compose, par. ext p. destruct p. reflexivity.
+Qed.
+
+Lemma par_comp :
+  forall (A B A' B' X : Type) (f : A -> B) (g : A' -> B') (h : B * B' -> X),
+    (f *** g) .> h = fun p : A * A' => h (f (fst p), g (snd p)).
+Proof.
+  intros. unfold compose, par. ext p. destruct p. cbn. reflexivity.
+Qed.
