Theory/Equivs/MonadComp.v
@@ -1,0 +1,36 @@
+Require Import HSLib.Base.
+
+Class Monad (M : Type -> Type) : Type :=
+{
+    pure : forall {A : Type}, A -> M A;
+    compM : forall {A B C : Type}, (A -> M B) -> (B -> M C) -> (A -> M C);
+    compM_pure_l :
+      forall (A B : Type) (f : A -> M B), compM pure f = f;
+    compM_pure_r :
+      forall (A B : Type) (f : A -> M B), compM f pure = f;
+    compM_assoc :
+      forall (A B C D : Type) (f : A -> M B) (g : B -> M C) (h : C -> M D),
+        compM f (compM g h) = compM (compM f g) h;
+}.
+
+Notation "f >=> g" := (compM f g) (at level 40).
+
+Definition bindM
+  (M : Type -> Type) (inst : Monad M)
+  {A B : Type} (x : M A) (f : A -> M B) : M B :=
+    compM (fun _ : unit => x) f tt.
+
+Hint Unfold bindM : HSLib.
+
+Require MonadBind.
+
+Instance Comp_to_Bind
+  (M : Type -> Type) (inst : Monad M) : MonadBind.Monad M :=
+{
+    bind := @bindM M inst;
+}.
+Proof.
+  all: MonadBind.monad.
+    apply pure. assumption.
+    Focus 2.
+Abort.
