Theory/Equivs/MonadEquiv.v
@@ -1,0 +1,82 @@
+Require Import Control.
+
+(*
+Module Join.
+Require Import MonadJoin.
+Require Import HSLib.Theory.Equivs.MonadJoin.
+Include HSLib.Theory.Equivs.MonadJoin.
+End Join.
+*)
+
+Module Join.
+Require MonadJoin.
+Include MonadJoin.
+End Join.
+
+Module Bind.
+Require MonadBind.
+Include MonadBind.
+End Bind.
+
+Module Comp.
+Require MonadComp.
+Include MonadComp.
+End Comp.
+
+(** * join-based definition *)
+
+Instance Join_to_Monad
+  (M : Type -> Type) (inst : Join.Monad M) : Monad M :=
+{
+    is_applicative := @Join.is_applicative M inst;
+    bind := @Join.bind M inst
+}.
+Proof.
+  apply Join.bind_pure_l.
+  apply Join.bind_pure_r.
+  apply Join.assoc.
+  apply Join.bind_ap.
+Defined.
+
+Instance Monad_to_Join (M : Type -> Type) (inst : Monad M)
+  : Join.Monad M :=
+{
+    is_applicative := @is_applicative M inst;
+    join := @join M inst
+}.
+Proof.
+  all: intros; unfold join, compose; try ext x.
+    rewrite bind_assoc, bind_fmap. unfold compose, id. reflexivity.
+    rewrite bind_pure_l. reflexivity.
+    rewrite bind_fmap, <- bind_pure_r. f_equal.
+    rewrite bind_fmap, fmap_bind. f_equal.
+    rewrite !bind_ap. monad.
+Defined.
+
+(** * bind-based definition *)
+
+Instance MonadBind_to_Monad
+  (M : Type -> Type) (inst : Bind.Monad M) : Monad M :=
+{
+    is_applicative := @MonadBind.MonadBind_to_Applicative M inst;
+    bind := @MonadBind.bind M inst;
+}.
+Proof. all: monad. Defined.
+
+Instance Monad_to_MonadBind
+  (M : Type -> Type) (inst : Monad M) : MonadBind.Monad M :=
+{
+    pure := @pure M inst;
+    bind := @bind M inst;
+}.
+Proof. all: monad. Defined.
+
+(** * compM-based definition *)
+
+Instance Monad_to_MonadComp
+  (M : Type -> Type) (inst : Monad M) : MonadComp.Monad M :=
+{
+    pure := @pure M inst;
+    compM := @compM M inst;
+}.
+Proof. all: unfold compM; monad. Defined.
