README.md
@@ -112,7 +112,7 @@ You can then compile the project at any time using `make` and recompile (for exa
 * Thievery:
   * Take a look at other Haskell proposals relating to the standard library design.
   * Browse Idris standard library and steal good stuff from there.
-  * Interesting Idris classes: Cast, Uninhabited, Sized
+  * Interesting Idris classes: Cast, Uninhabited, Sized, Read
 
 ### Particular
 
@@ -129,8 +129,9 @@ You can then compile the project at any time using `make` and recompile (for exa
 * Check if the law `fmap_pure_ap` is necessary for Applicative.
 * Something practical: maybe use the monadic stuff for Enumerable/Finite classes.
 * Check what is the precise relation between bind and ap (and if it's possible to define monads in two nonequivalent ways due to this).
+* Check if the Lazy monad makes sense.
+* Decide what to do with ContT and ContT_refactored.
 
 ### Technical
 
 * Revise the compilation steps from this README file.
-* Rename all objects that contain 'wut' in their names.
