make_makefile.sh
@@ -1,7 +1,5 @@
 #!/bin/sh
 
-#coq_makefile -R "." HSLib -o makefile Base.v Alternative/**v Applicative Functor Instances InstancesT MonadBind MonadComp MonadJoin MonadPlus MonadTrans
+#coq_makefile -R "." HSLib -o makefile **v */**v
 
-coq_makefile -R "." HSLib -o makefile **v */**v
-
-#coq_makefile -R "." RandomCoqCode -o makefile RCCBase.v Reflection/**v Sorting/**v Structures/**v Trash/**v Trees/**v
+coq_makefile -R "." HSLib -o makefile *v Control/*v Instances/*v InstancesT/*v Misc/*v MonadClass/*v Parser/*v Tactics/*v Theory/*v Theory/Laws/*v Theory/Equivs/*v
